Further work on theories
Have internal and external context, namespace,
lemmas/axioms, and validity predicate

Need to generate proof goals, then test/use this
to debug

proofs/core/Theory.v
@@ -33,33 +33,22 @@ with theory_rec := Induction for theory Sort Type.
 Check tdecl_rec.*)
 (*ALT (maybe better) - use old, use Equations with size measure
 better - define size of tdecl, lift to list, use as measure*)
-(*Induction principle not good for this one*)
-Inductive tdecl : Set :=
-  | tdef : def -> tdecl
-  | tprop : prop_kind -> string -> formula -> tdecl
-  (*Use a theory (copy all of its definitions).
-    Bool represents if exported or not*)
-  | tuse : list tdecl -> bool -> tdecl
-  (*Clone a theory - instantiating some parameters and giving
-    a qualified name*)
-  | tclone: list tdecl -> string -> list (typesym * typesym) ->
-    list (funsym * funsym) -> list (predsym * predsym) -> bool -> tdecl.
 
-Definition theory : Set := list tdecl.
-
-(*To write inductive functions over theories that
-  recurse as we expect (into tuse and tclone), we define a 
-  notion of "size"*)
-Fixpoint tdecl_size (t: tdecl) : nat :=
-  match t with
-  | tdef d => 1
-  | tprop _ _ _ => 1
-  | tuse ts _ => 1 + sum (map tdecl_size ts)
-  | tclone ts _ _ _ _ _ => 1 + sum (map tdecl_size ts)
-  end.
-
-Definition theory_size (t: theory) : nat :=
-  sum (map tdecl_size t).
+(*We require 2 additional restrictions that why3 does not have
+  (at least for now)
+  1. All "clone"d theories must be exported
+  2. All "clone"d theories must use qualified names
+  
+  With these restrictions, we can define notions of well-typed
+  and valid theories and we can check these efficiently.
+  In particular, we can identify all of the theories "use"d in
+  a theory T and require that if we use/clone T in A, as long
+  as we use all the same theories that T depends on, the
+  resulting theory A is well-typed/proved.
+  This means that we do not need to re-check things that
+  we have already typed/verified, which is crucial for 
+  performance and modularity
+  *)
 
 (*We can view theories as comprising 2 things:
   A context (formed by the definitions as well as the uses
@@ -73,8 +62,9 @@ Definition theory_size (t: theory) : nat :=
   To do this, we separate the context formed from
   a given theory into the internal context (what we need
     to prove things, expanding all "use" and "clone")
-  and the external one, which only includes "use"s and "clone"s
-  marked as exported
+  and the external one, which only includes "use"s
+  marked as exported (all "clone"s are exported in our
+  system)
   *)
 
 (*Substitution*)
@@ -260,38 +250,395 @@ Definition sub_ctx_map (c: context)  :
     end
   ) nil c.
 
+(*Substitute according to map in list of (string * formula)*)
+Definition sub_props_map (l: list (string * formula)) : list (string * formula) :=
+  map (fun x => (fst x, (sub_in_f (snd x)))) l.
+
 End Sub.
 
-Print tdecl.
+(*From why3 theory.ml - they use string -> typesym, etc maps
+  I should too, eventually*)
+Record namespace := mk_ns {
+  ns_ts: list (string * typesym);
+  ns_fs: list (string * funsym);
+  ns_ps: list (string * predsym)
+}.
 
-(*The external context of a theory*)
+Definition ts_in_ns (t: typesym) (n: namespace) : bool :=
+  match (get_assoc_list string_dec (ns_ts n) (ts_name t) ) with
+  | Some t1 => typesym_eq_dec t t1
+  | None => false
+  end.
 
-(*TODO: need to implement qualified names*)
+Definition fs_in_ns (f: funsym) (n: namespace) : bool :=
+  match (get_assoc_list string_dec (ns_fs n) (s_name f) ) with
+  | Some f1 => funsym_eq_dec f f1
+  | None => false
+  end.
 
-#[local] Instance theory_size_wf:
-Classes.WellFounded
-        (Telescopes.tele_measure (Telescopes.tip theory) nat
-           (fun t : theory => theory_size t) lt).
-unfold Classes.WellFounded, Telescopes.tele_measure. simpl.
-apply Inverse_Image.wf_inverse_image.
-apply Nat.lt_wf_0.
-Defined.
+Definition ps_in_ns (p: predsym) (n: namespace) : bool :=
+  match (get_assoc_list string_dec (ns_ps n) (s_name p) ) with
+  | Some p1 => predsym_eq_dec p p1
+  | None => false
+  end.
 
-(*Solves all goals*)
-Obligation Tactic := intros; try (unfold theory_size); simpl; try lia.
+(*Qualified names*)
+Section QualNames.
 
-(*We use Equations because this is not obviously stucturally
-  recursive (or at least Coq cannot tell that it is)*)
+(*Change all top-level type, function, and predicate
+  definitions to use a qualified prefix*)
+Variable prefix : string.
+
+Variable n: namespace.
+Local Open Scope string_scope.
+Definition add_prefix (s: string) := prefix ++ "."%string ++ s.
+
+Definition qual_ts (t: typesym) : typesym :=
+  mk_ts (add_prefix (ts_name t)) (ts_args t).
+
+Definition qual_ts_n (t: typesym) : typesym :=
+  if ts_in_ns t n then qual_ts t else t.
+
+Fixpoint qual_vty (v: vty) : vty :=
+  match v with
+  | vty_int => vty_int
+  | vty_real => vty_real
+  | vty_var x => vty_var x
+  | vty_cons ts vs => vty_cons (qual_ts_n ts) (map qual_vty vs)
+  end.
+
+Lemma qual_vty_vars t:
+  type_vars (qual_vty t) = type_vars t.
+Proof.
+  induction t; simpl; auto.
+  induction vs; simpl; auto.
+  inversion H; subst.
+  rewrite H2. f_equal. auto.
+Qed.
+
+Lemma check_args_qual {params args}:
+  check_args params args ->
+  check_args params (map qual_vty args).
+Proof.
+  unfold is_true.
+  rewrite <- !(reflect_iff _ _ (check_args_correct _ _)); intros.
+  unfold sublist in *.
+  intros.
+  rewrite in_map_iff in H0.
+  destruct H0 as [t [Ht Hint]]; subst.
+  rewrite qual_vty_vars in H1.
+  apply (H _ Hint); auto.
+Qed.
+
+Lemma check_sublist_qual {t params}:
+  check_sublist (type_vars t) params ->
+  check_sublist (type_vars (qual_vty t)) params.
+Proof.
+  rewrite qual_vty_vars; auto.
+Qed.
+
+Definition qual_fpsym (f: fpsym) : fpsym :=
+  Build_fpsym (add_prefix (s_name f)) (s_params f)
+    (map qual_vty (s_args f)) (check_args_qual (s_args_wf f)) 
+    (s_params_nodup f).
+
+Definition qual_funsym (f: funsym) : funsym :=
+  Build_funsym (qual_fpsym (f_sym f))
+    (qual_vty (f_ret f))
+    (check_sublist_qual (f_ret_wf f)).
+
+Definition qual_funsym_n (f: funsym) : funsym :=
+  if fs_in_ns f n then f else qual_funsym f.
+
+Definition qual_predsym (p: predsym) : predsym :=
+  Build_predsym (qual_fpsym p).
+
+Definition qual_predsym_n (p: predsym) : predsym :=
+  if ps_in_ns p n then p else qual_predsym p.
+
+Definition qual_alg_datatype (a: alg_datatype) : alg_datatype :=
+  match a with
+  | alg_def ts fs => alg_def (qual_ts ts) (map_ne_list qual_funsym_n fs)
+  end.
+
+Definition qual_mut_adt (m: mut_adt) : mut_adt :=
+  mk_mut (map qual_alg_datatype (typs m)) (m_params m)
+  (m_nodup m).
+
+Definition qual_vs (x: vsymbol) : vsymbol :=
+  (fst x, qual_vty (snd x)).
+
+Fixpoint qual_pat (p: pattern) : pattern :=
+  match p with
+  | Pvar v => Pvar (qual_vs v)
+  | Pconstr fs tys pats => Pconstr (qual_funsym_n fs) (map qual_vty tys)
+    (map qual_pat pats)
+  | Pwild => Pwild
+  | Por p1 p2 => Por (qual_pat p1) (qual_pat p2)
+  | Pbind p x => Pbind (qual_pat p) (qual_vs x)
+  end.
+  
+Fixpoint qual_tm (t: term) : term :=
+  match t with
+  | Tconst c => Tconst c
+  | Tvar v => Tvar (qual_vs v)
+  | Tfun fs tys tms => Tfun (qual_funsym_n fs) (map qual_vty tys) 
+    (map qual_tm tms)
+  | Tlet t1 v t2 => Tlet (qual_tm t1) (qual_vs v) (qual_tm t2)
+  | Tif f t1 t2 => Tif (qual_fmla f) (qual_tm t1) (qual_tm t2)
+  | Tmatch t v ps => Tmatch (qual_tm t) (qual_vty v)
+    (map (fun x => (qual_pat (fst x), qual_tm (snd x))) ps)
+  | Teps f v => Teps (qual_fmla f) (qual_vs v)
+  end
+with qual_fmla (f: formula) : formula :=
+  match f with
+  | Fpred p tys tms => Fpred (qual_predsym_n p) (map qual_vty tys)
+    (map qual_tm tms)
+  | Fquant q v f => Fquant q (qual_vs v) (qual_fmla f)
+  | Feq ty t1 t2 => Feq (qual_vty ty) (qual_tm t1) (qual_tm t2)
+  | Fbinop b f1 f2 => Fbinop b (qual_fmla f1) (qual_fmla f2)
+  | Fnot f => Fnot (qual_fmla f)
+  | Ftrue => Ftrue
+  | Ffalse => Ffalse
+  | Flet t v f => Flet (qual_tm t) (qual_vs v) (qual_fmla f)
+  | Fif f1 f2 f3 => Fif (qual_fmla f1) (qual_fmla f2) (qual_fmla f3)
+  | Fmatch t v ps => Fmatch (qual_tm t) (qual_vty v)
+    (map (fun x => (qual_pat (fst x), qual_fmla (snd x))) ps)
+  end.
+
+Definition qual_funpred_def (f: funpred_def) : funpred_def :=
+  match f with
+  | fun_def f xs t => fun_def (qual_funsym_n f) (map qual_vs xs) (qual_tm t)
+  | pred_def p xs f => pred_def (qual_predsym_n p) (map qual_vs xs)
+    (qual_fmla f)
+  end.
+
+Definition qual_indpred_def (i: indpred_def) : indpred_def :=
+  match i with
+  | ind_def p xs => ind_def (qual_predsym_n p) 
+    (map (fun x => (add_prefix (fst x), qual_fmla (snd x))) xs)
+  end.
+
+Definition qual_def (d: def) : def :=
+  match d with
+  | datatype_def m => datatype_def (qual_mut_adt m)
+  | recursive_def l => recursive_def (map qual_funpred_def l)
+  | inductive_def i => inductive_def (map qual_indpred_def i)
+  | abs_type ts => abs_type (qual_ts_n ts)
+  | abs_fun f => abs_fun (qual_funsym_n f)
+  | abs_pred p => abs_pred (qual_predsym_n p)
+  end.
+
+End QualNames.
+
+
+(*Get all definitions from a theory*)
+
+(*Problem - to get definition, need to have qualified names*)
+
+
+(*Here's what I will do:
+  theory will be mutually recursive with tdecl
+  theory consists of list tdecl, list typesym, list funsym,
+    list predsym
+  these lists represent the (external) namespace of the the
+  theory
+
+  then, qualify a theory as follows:
+  identify all of the "uses" in the theory and look at 
+  all of their lists
+  qualify everything in the theory EXCEPT for the things
+  in this list
+  (and update the external lists appropriately)
+  alternatively, update lists first, qualify everything IN list
+
+  then, to get context of theory, qualify "clones" using this
+
+  this solves the problem of circular dependencies
+
+  problem before: qualify theory -> need names to
+    (not) qualify, look through "use", need to qualify
+    inner theories - here, dont have functions, store data,
+    assume populated correctly and we will ensure that this
+    is the case
+
+*)
+
+
+
+(*
+Unset Elimination Schemes.
+*)
+Inductive tdecl : Set :=
+  | tdef : def -> tdecl
+  | tprop : prop_kind -> string -> formula -> tdecl
+  (*Use a theory (copy all of its definitions).
+    Bool represents if exported or not*)
+  | tuse : list tdecl -> bool -> tdecl
+  (*Clone a theory - instantiating some parameters and giving
+    a qualified name*)
+  | tclone: list tdecl -> string -> list (typesym * typesym) ->
+    list (funsym * funsym) -> list (predsym * predsym) -> tdecl.
+
+Definition theory := list tdecl.
+(*
+with theory : Set :=
+  | mk_theory : list tdecl -> namespace -> theory.
+
+Scheme tdecl_ind := Induction for tdecl Sort Prop
+  with theory_ind := Induction for theory Sort Prop.
+Scheme tdecl_rec := Induction for tdecl Sort Type
+  with theory_rec := Induction for theory Sort Type.
+Set Elimination Schemes.*)
+
+(*Qualify names in a theory*)
+
+(*Definition th_export (t: theory) : namespace :=
+  match t with
+  | mk_theory _ n => n
+  end.*)
+
+
+(*To write inductive functions over theories that
+  recurse as we expect (into tuse and tclone), we define a 
+  notion of "size"*)
+  Fixpoint tdecl_size (t: tdecl) : nat :=
+    match t with
+    | tdef d => 1
+    | tprop _ _ _ => 1
+    | tuse ts _ => 1 + sum (map tdecl_size ts)
+    | tclone ts _ _ _ _ => 1 + sum (map tdecl_size ts)
+    end.
+  
+  Definition theory_size (t: theory) : nat :=
+    sum (map tdecl_size t).
+  
+  
+  
+  (*We use Equations because we write functions that are
+    not obviously stucturally
+    recursive (or at least Coq cannot tell that they are)*)
+  
+  (* #[local] Instance theory_size_wf:
+  Classes.WellFounded
+          (Telescopes.tele_measure (Telescopes.tip theory) nat
+             (fun t : theory => theory_size t) lt).
+  unfold Classes.WellFounded, Telescopes.tele_measure. simpl.
+  apply Inverse_Image.wf_inverse_image.
+  apply Nat.lt_wf_0.
+  Defined.*)
+  
+  From Equations Require Import Equations.
+  (*Solves all goals*)
+  Obligation Tactic := intros; try (unfold theory_size); simpl; try lia.
+  
+  (*We need a bunch of utilities*)
+(*Utilities for namespace (move)*)
+Definition emp_namespace : namespace :=
+  mk_ns nil nil nil.
+
+Definition add_ts_to_ns (tss: list typesym) (n: namespace) : namespace :=
+  mk_ns (map (fun x => (ts_name x, x)) tss ++ (ns_ts n)) (ns_fs n) (ns_ps n).
+
+Definition add_fs_to_ns (fss: list funsym) (n: namespace) : namespace :=
+  mk_ns (ns_ts n) (map (fun (x: funsym) => (s_name x, x)) fss ++ (ns_fs n))
+    (ns_ps n).
+
+Definition add_ps_to_ns (pss: list predsym) (n: namespace) : namespace :=
+  mk_ns (ns_ts n) (ns_fs n) 
+  (map (fun (x: predsym) => (s_name x, x)) pss ++ (ns_ps n)).
+
+Definition add_def_to_ns (d: def) (n: namespace) : namespace :=
+  add_ps_to_ns (predsyms_of_def d) 
+    (add_fs_to_ns (funsyms_of_def d)
+      (add_ts_to_ns (typesyms_of_def d) n)).
+
+(*TODO: should really be union*)
+Definition merge_ns (n1 n2: namespace) : namespace :=
+  mk_ns ((ns_ts n1) ++ (ns_ts n2)) ((ns_fs n1) ++ (ns_fs n2))
+    ((ns_ps n1) ++ (ns_ps n2)).
+
+(*Add s as prefix to all entries in namespace*)
+Definition qualify_all (s: string) (n: namespace) : namespace :=
+  mk_ns (map (fun x => (add_prefix s (fst x), qual_ts_n s n (snd x))) (ns_ts n))
+    (map (fun x => (add_prefix s (fst x), qual_funsym_n s n (snd x))) (ns_fs n))
+    (map (fun x => (add_prefix s (fst x), qual_predsym_n s n (snd x))) (ns_ps n)).
+
+
+
+(*Get all exported names (only) from a theory*)
+Equations get_exported_names (t: theory) : namespace 
+  by wf (theory_size t) lt :=
+get_exported_names nil := emp_namespace;
+get_exported_names (tdef d :: tl) := 
+  add_def_to_ns d (get_exported_names tl);
+get_exported_names (tprop _ _ _ :: tl) := get_exported_names tl;
+get_exported_names (tuse th true :: tl) := 
+  merge_ns (get_exported_names th) (get_exported_names tl);
+get_exported_names (tuse th false :: tl) := get_exported_names tl;
+get_exported_names (tclone th s tys funs preds :: tl) :=
+  merge_ns (qualify_all s (get_exported_names th)) (get_exported_names tl)
+.
+
+Definition add_qual (s1 s2: string) :=
+  (s1 ++ "."%string ++ s2)%string.
+
+
+(*Now we can qualify a theory - replace all exported definitions
+  and uses of these definitions (BUT NOT used-but-not-exported defs)
+  with qualified symbols*)
+Equations qualify_theory (s: string) (n: namespace) (t: theory) : theory 
+  by wf (theory_size t) lt :=
+qualify_theory s n nil := nil;
+qualify_theory s n (tdef d :: tl) := 
+  tdef (qual_def s n d) :: qualify_theory s n tl;
+qualify_theory s n (tprop k name f :: tl) :=
+  (tprop k (add_prefix s name) (qual_fmla s n f)) :: tl;
+(*A used theory that is exported is qualified - we add all qualified
+  defs to our theory*)
+qualify_theory s n (tuse th true :: tl) :=
+  tuse (qualify_theory s n th) true :: qualify_theory s n tl;
+(*If not used, don't add*)
+qualify_theory s n (tuse th false :: tl) := qualify_theory s n tl;
+(*Cloned theories are qualified first, then qualified again (see)*)
+qualify_theory s n (tclone th name tys funs preds :: tl) :=
+  tclone (qualify_theory (add_qual s name) n th) name (*TODO: qualify name?*)
+    tys funs preds :: qualify_theory s n tl
+  .
+
+Set Bullet Behavior "Strict Subproofs".
+
+(*Qualified theory has same size*)
+Lemma qualify_theory_size (s: string) (n: namespace) (t: theory) :
+  theory_size (qualify_theory s n t) <= theory_size t.
+Proof.
+  revert s n t.
+  apply (qualify_theory_elim (fun s n t1 t2 => theory_size t2 <= theory_size t1));
+  simpl; intros; auto; unfold theory_size in *; simpl; lia.
+Qed.
+
+(*Now, we can get the internal and external context of a theory.
+  We also give the exported axioms and lemmas*)
+
 Equations theory_ctx_ext (t: theory) : context
   by wf (theory_size t) lt :=
 theory_ctx_ext (tdef d :: tl) := d :: theory_ctx_ext tl;
 theory_ctx_ext (tuse l true :: tl) :=
   (*Not structurally recursive*)
   theory_ctx_ext l ++ theory_ctx_ext tl;
-theory_ctx_ext (tclone l _ tys funs preds true :: tl) :=
-  sub_ctx_map tys funs preds (theory_ctx_ext l) ++ theory_ctx_ext tl;
+theory_ctx_ext (tclone l name tys funs preds :: tl) :=
+  (*for a clone, we first get the exported names to qualify, then
+    we qualify, then we sub in (so the sub takes the qualified names)*)
+  let n := get_exported_names l in
+  let qual := qualify_theory name n l in 
+  sub_ctx_map tys funs preds (theory_ctx_ext qual) ++ theory_ctx_ext tl;
 theory_ctx_ext (_ :: tl) := theory_ctx_ext tl;
 theory_ctx_ext nil := nil.
+Next Obligation.
+subst qual.
+pose proof (qualify_theory_size name n l). 
+unfold theory_size in *. lia.
+Defined.
 
 (*And the internal theory context - only use external context
   of imported modules - this one is structurally recursive*)
@@ -300,8 +647,10 @@ Fixpoint theory_ctx_int (t: theory) : context :=
   | tdef d :: tl => d :: theory_ctx_int tl
   | tuse l true :: tl =>
       theory_ctx_ext l ++ theory_ctx_int tl
-  | tclone l _ tys funs preds _ :: tl =>
-    sub_ctx_map tys funs preds (theory_ctx_ext l) ++ theory_ctx_int tl
+  | tclone l name tys funs preds  :: tl =>
+    let n := get_exported_names l in
+    let qual := qualify_theory name n l in 
+    sub_ctx_map tys funs preds (theory_ctx_ext qual) ++ theory_ctx_int tl
   | _ :: tl => theory_ctx_int tl
   | nil => nil
   end.
@@ -320,3 +669,168 @@ Fixpoint theory_ctx_int (t: theory) : context :=
   previous axioms/lemmas - then valid iff all tasks are valid
   give as Inductive and Fixpoint (for generating goals) most likely
   *)
+
+(*Well-typed theory*)
+Definition typed_theory (t: theory) : Prop :=
+  valid_context (theory_ctx_int t).
+
+(*Typechecking*)
+
+(*We want to check efficiently, not having to check the whole
+  context. So we give an alternate definition of a typed theory,
+  which we show is equivalent to the original one*)
+(*  Print valid_context.
+Require Import Typechecker.
+Print tdecl.
+(*Suppose we have already typechecked all of the
+  external theories that we "use" and "clone".
+  Then, we don't want to typecheck them again*)
+
+(*TODO: for now, just typecheck things again. But
+  we should REALLY go back and implement this fully*)
+
+
+Fixpoint check_typed_theory (t: theory) : bool :=
+  match t with
+  | nil => true
+  | h :: tl =>
+    check_typed_theory_tl &&
+    match h with
+    | tdef d =>
+      (*TODO: expensive to get context every time*)
+      check_context_cons d (theory_ctx_int t)
+    | tprop p name f =>
+      (*Typecheck prop formula - or TODO - do with valid?*)
+      typecheck_formula f (theory_ctx_int t)
+    | tuse th b =>
+      (**)
+
+
+    check_typed_theory_tl
+  end.
+*)
+
+(*Valid theory*)
+
+(*To show that a theory is valid, we generate a series of tasks
+  in the way that we might expect: go through the theory and
+  prove each lemma/goal, assuming all previous axioms/lemmas*)
+
+Require Import Task.
+
+
+
+(*Axioms/lemmas from a theory that can be used externally*)
+Equations theory_axioms_ext (t: theory) : list (string * formula) 
+  by wf (theory_size t) lt :=
+(*Add lemmas and axioms from current theory*)
+theory_axioms_ext (tprop Paxiom name f :: tl)  :=
+  (name, f) :: theory_axioms_ext tl;
+theory_axioms_ext (tprop Plemma name f :: tl) :=
+  (name, f) :: theory_axioms_ext tl;
+(*Add all from used that we export*)
+theory_axioms_ext (tuse th true :: tl) :=
+  theory_axioms_ext th ++ theory_axioms_ext tl;
+(*Add all from cloning, after qualifying and substituting*)
+theory_axioms_ext (tclone th name tys funs preds :: tl) :=
+  let n := get_exported_names th in
+  (*This also qualifies props*)
+  let qual := qualify_theory name n th in
+  sub_props_map tys funs preds (theory_axioms_ext qual) ++
+  theory_axioms_ext tl;
+(*No other lemmas/axioms*)
+theory_axioms_ext nil := nil;
+theory_axioms_ext (_ :: tl) := theory_axioms_ext tl.
+Next Obligation.
+subst qual.
+pose proof (qualify_theory_size name n th). 
+unfold theory_size in *. lia.
+Defined.
+
+(*Difference - we are allowed to use theorems in "use"*)
+Fixpoint theory_axioms_int (t: theory) : list (string * formula) :=
+  match t with
+  | tprop Paxiom name f :: tl =>
+    (name, f) :: theory_axioms_int tl
+  | tprop Plemma name f :: tl =>
+    (name, f) :: theory_axioms_int tl
+  | tuse th _ :: tl =>
+    theory_axioms_ext th ++ theory_axioms_ext tl
+  | tclone th name tys funs preds :: tl =>
+    let n := get_exported_names th in
+    let qual := qualify_theory name n th in 
+    sub_props_map tys funs preds (theory_axioms_ext qual) ++ 
+    theory_axioms_int tl
+  | _ :: tl => theory_axioms_int tl
+  | nil => nil
+  end.
+Print tdecl.
+
+(*This defines what it means for a theory
+  to be valid.
+  We want to do the following
+  1. Give a function that generates proof goals 
+    to prove that a theory is valid
+  2. Maybe give typeclasses to help with proving
+    dependencies
+  3. Prove that this definition implies that,
+    for a given theory t and formula f,
+    if we have (valid_theory (tprop Plemma/Pgoal _ f :: t)),
+    then (theory_ctx_int t, theory_axioms t) |= f
+    and as a corollary, if no axioms, then gamma, . |= f
+    (more of a sanity check than anything else)*)
+Inductive valid_theory : theory -> Prop :=
+  | valid_th_emp: valid_theory nil
+  | valid_th_def: forall d t,
+    valid_theory t ->
+    (*The context with this def is well-typed*)
+    valid_context (d :: theory_ctx_int t) ->
+    valid_theory (tdef d :: t)
+  (*For axioms, only need to check type I think*)
+  | valid_th_axiom: forall name f t,
+    valid_theory t ->
+    formula_typed (theory_ctx_int t) f ->
+    valid_theory (tprop Paxiom name f :: t)
+  | valid_th_lemma: forall name f t,
+    valid_theory t ->
+    (*We build the task consisting of the context
+      of the theory, the assumptions so far, and the 
+      goal*)
+    let tsk := mk_task (theory_ctx_int t)
+      (map snd (theory_axioms_int t)) nil f in
+    (*The task must be well-typed*)
+    task_wf tsk ->
+    (*The task must be valid*)
+    (forall (wf: task_wf tsk),
+      task_valid tsk wf) ->
+    valid_theory (tprop Plemma name f :: t)
+  (*goals are identical*)
+  | valid_th_goal: forall name f t,
+    valid_theory t ->
+    (*We build the task consisting of the context
+      of the theory, the assumptions so far, and the 
+      goal*)
+    let tsk := mk_task (theory_ctx_int t)
+      (map snd (theory_axioms_int t)) nil f in
+    (*The task must be well-typed*)
+    task_wf tsk ->
+    (*The task must be valid*)
+    (forall (wf: task_wf tsk),
+      task_valid tsk wf) ->
+    valid_theory (tprop Pgoal name f :: t)
+  (*For "use", just need existing theory to be valid*)
+  | valid_th_use: forall th b t,
+    valid_theory t ->
+    valid_theory th ->
+    valid_theory (tuse th b :: t)
+  (*And similarly for clone, but we need to ensure that
+    the things that we substitute are valid (TODO: in typing?)*)
+  | valid_th_clone: forall th name tys funs preds t,
+    valid_theory t ->
+    valid_theory th ->
+    let gamma := theory_ctx_int t in
+    (forall ty, In ty (map snd tys) -> In ty (sig_t gamma)) ->
+    (forall f, In f (map snd funs) -> In f (sig_f gamma)) ->
+    (forall p, In p (map snd preds) -> In p (sig_p gamma)) ->
+    valid_theory (tclone th name tys funs preds :: t).
+
